new cast compat lemmas, well-typeness back expr, small fixes

theories/backtranslation/cast_help/factorize.v
@@ -16,50 +16,72 @@ Qed.
 
 (** Factorisations *)
 
-Definition factorization_up (f : expr) (τG : cast_calculus.types.type) (G : Ground τG) : val :=
+Definition factorization (f g : expr) : val :=
   LamV (
-      embed τG G (f.[ren (+1)] (Var 0))
+      g.[ren (+1)] (f.[ren (+1)] (Var 0))
     ).
 
-Lemma factorization_up_subst_rewrite (f : expr) (τG : cast_calculus.types.type) (G : Ground τG) σ : (# (factorization_up f τG G)).[σ] = factorization_up f.[σ] τG G.
-Proof.
-  rewrite /factorization_up.
-  asimpl. by rewrite embed_no_subs.
-Qed.
+Lemma factorization_subst_rewrite (f g : expr) σ : (# (factorization f g)).[σ] = factorization f.[σ] g.[σ].
+Proof. by asimpl. Qed.
 
-Lemma factorization_up_typed Γ pΓ {f : expr} (τ : type) pτ (τG : cast_calculus.types.type) (G : Ground τG)
-      (d : Γ & pΓ ⊢ₛ f : (TArrow τ <<τG>>) & TArrow_closed pτ (back_Ground_closed G)) :
-  Γ & pΓ ⊢ₛ factorization_up f τG G : (TArrow τ Universe) & TArrow_closed pτ Universe_closed.
+Lemma factorization_typed Γ pΓ {f g : expr} (τ1 : type) pτ1 τ2 pτ2 τ3 pτ3
+      (df : Γ & pΓ ⊢ₛ f : (TArrow τ1 τ2) & TArrow_closed pτ1 pτ2)
+      (dg : Γ & pΓ ⊢ₛ g : (TArrow τ2 τ3) & TArrow_closed pτ2 pτ3) :
+  Γ & pΓ ⊢ₛ factorization f g : (TArrow τ1 τ3) & TArrow_closed pτ1 pτ3.
 Proof.
   eapply Lam_typed.
-  eapply App_typed with (τ1 := << τG >>).
-  apply embed_typed.
-  eapply App_typed with (τ1 := τ ).
-  eapply up_type_one. apply d.
+  eapply App_typed with (τ1 := τ2).
+  eapply up_type_one. apply dg.
+  eapply App_typed with (τ1 := τ1).
+  eapply up_type_one. apply df.
   by apply Var_typed.
-  Unshelve. all:(auto||apply Universe_closed||by apply back_Ground_closed).
+  Unshelve. all:auto.
 Qed.
 
-Definition factorization_down (f : expr) (τG : cast_calculus.types.type) (G : Ground τG) : val :=
-  LamV (
-      (f.[ren (+1)]) (extract τG G (Var 0))
-    ).
+(* Definition factorization_up (f : expr) (τG : cast_calculus.types.type) (G : Ground τG) : val := *)
+(*   LamV ( *)
+(*       embed τG G (f.[ren (+1)] (Var 0)) *)
+(*     ). *)
 
-Lemma factorization_down_subst_rewrite (f : expr) (τG : cast_calculus.types.type) (G : Ground τG) σ : (# (factorization_down f τG G)).[σ] = factorization_down f.[σ] τG G.
-Proof.
-  rewrite /factorization_down.
-  asimpl. by rewrite extract_no_subs.
-Qed.
+(* Lemma factorization_up_subst_rewrite (f : expr) (τG : cast_calculus.types.type) (G : Ground τG) σ : (# (factorization_up f τG G)).[σ] = factorization_up f.[σ] τG G. *)
+(* Proof. *)
+(*   rewrite /factorization_up. *)
+(*   asimpl. by rewrite embed_no_subs. *)
+(* Qed. *)
 
-Lemma factorization_down_typed Γ pΓ {f : expr} (τ : type) pτ (τG : cast_calculus.types.type) (G : Ground τG)
-      (d : Γ & pΓ ⊢ₛ f : (TArrow <<τG>> τ) & (TArrow_closed (back_Ground_closed G) pτ)) :
-  Γ & pΓ ⊢ₛ factorization_down f τG G : (TArrow Universe τ) & (TArrow_closed Universe_closed pτ).
-Proof.
-  eapply Lam_typed.
-  eapply App_typed with (τ1 := << τG >>).
-  eapply up_type_one. apply d.
-  eapply App_typed with (τ1 := Universe).
-  apply extract_typed.
-  by apply Var_typed.
-  Unshelve. all:(auto||apply Universe_closed||by apply back_Ground_closed).
-Qed.
+(* Lemma factorization_up_typed Γ pΓ {f : expr} (τ : type) pτ (τG : cast_calculus.types.type) (G : Ground τG) *)
+(*       (d : Γ & pΓ ⊢ₛ f : (TArrow τ <<τG>>) & TArrow_closed pτ (back_Ground_closed G)) : *)
+(*   Γ & pΓ ⊢ₛ factorization_up f τG G : (TArrow τ Universe) & TArrow_closed pτ Universe_closed. *)
+(* Proof. *)
+(*   eapply Lam_typed. *)
+(*   eapply App_typed with (τ1 := << τG >>). *)
+(*   apply embed_typed. *)
+(*   eapply App_typed with (τ1 := τ ). *)
+(*   eapply up_type_one. apply d. *)
+(*   by apply Var_typed. *)
+(*   Unshelve. all:(auto||apply Universe_closed||by apply back_Ground_closed). *)
+(* Qed. *)
+
+(* Definition factorization_down (f : expr) (τG : cast_calculus.types.type) (G : Ground τG) : val := *)
+(*   LamV ( *)
+(*       (f.[ren (+1)]) (extract τG G (Var 0)) *)
+(*     ). *)
+
+(* Lemma factorization_down_subst_rewrite (f : expr) (τG : cast_calculus.types.type) (G : Ground τG) σ : (# (factorization_down f τG G)).[σ] = factorization_down f.[σ] τG G. *)
+(* Proof. *)
+(*   rewrite /factorization_down. *)
+(*   asimpl. by rewrite extract_no_subs. *)
+(* Qed. *)
+
+(* Lemma factorization_down_typed Γ pΓ {f : expr} (τ : type) pτ (τG : cast_calculus.types.type) (G : Ground τG) *)
+(*       (d : Γ & pΓ ⊢ₛ f : (TArrow <<τG>> τ) & (TArrow_closed (back_Ground_closed G) pτ)) : *)
+(*   Γ & pΓ ⊢ₛ factorization_down f τG G : (TArrow Universe τ) & (TArrow_closed Universe_closed pτ). *)
+(* Proof. *)
+(*   eapply Lam_typed. *)
+(*   eapply App_typed with (τ1 := << τG >>). *)
+(*   eapply up_type_one. apply d. *)
+(*   eapply App_typed with (τ1 := Universe). *)
+(*   apply extract_typed. *)
+(*   by apply Var_typed. *)
+(*   Unshelve. all:(auto||apply Universe_closed||by apply back_Ground_closed). *)
+(* Qed. *)
