theories/backtranslation/well_typedness.v
@@ -1,70 +1,89 @@
-From fae_gtlc_mu.cast_calculus Require Export typing contexts.
-From fae_gtlc_mu.stlc_mu Require Export typing contexts.
+From fae_gtlc_mu.cast_calculus Require Export typing (*contexts*).
+From fae_gtlc_mu.stlc_mu Require Export typing (*contexts*).
 
-From fae_gtlc_mu.backtranslation Require Import types expressions cast_help.general contexts.
+From fae_gtlc_mu.backtranslation Require Import types expressions cast_help.general (*contexts*).
 
-Lemma well_typedness_expr Γ e τ :
-  Γ ⊢ₜ e : τ →
-    map backtranslate_type Γ ⊢ₛ backtranslate_expr e : backtranslate_type τ.
+Lemma force_typed Γ Γ' pΓ pΓ' e τ τ' pτ pτ' : Γ & pΓ ⊢ₛ e : τ & pτ → Γ = Γ' → τ = τ' → Γ' & pΓ' ⊢ₛ e : τ & pτ'. (** use with cae *)
+Proof. intros. simplify_eq. eapply PI_typed. eapply PI_Γ_typed. done. Qed.
+
+Lemma well_typedness_expr Γ pΓ e τ pτ :
+  Γ & pΓ ⊢ₜ e : τ & pτ →
+    map backtranslate_type Γ & (Forall_fmap_impl _ _ _ _ (@back_closed) pΓ) ⊢ₛ backtranslate_expr e : backtranslate_type τ & (back_closed pτ).
 Proof.
-  induction 1; simpl; try by constructor.
+  induction 1; simpl; try by econstructor.
   - constructor. by rewrite list_lookup_fmap H.
-  - eapply Fst_typed. apply IHtyped.
-  - eapply Snd_typed. apply IHtyped.
-  - eapply Case_typed. apply IHtyped1. apply IHtyped2. apply IHtyped3.
-  - eapply App_typed. apply IHtyped1. apply IHtyped2.
-  - apply Fold_typed.
-    rewrite unfolding_backtranslation_commutes in IHtyped.
-    apply IHtyped.
-  - rewrite unfolding_backtranslation_commutes.
-    apply Unfold_typed. apply IHtyped.
-  - destruct (cons_stand_dec τi τf); destruct (decide (TClosed τi)); destruct (decide (TClosed τf)); try by contradiction.
+  - eapply Case_typed. apply IHtyped1.
+    eapply PI_typed. eapply PI_Γ_typed. apply IHtyped2.
+    eapply PI_typed. eapply PI_Γ_typed. apply IHtyped3.
+  - eapply Lam_typed. eapply PI_Γ_typed. apply IHtyped.
+  - assert (HC : TClosed <<(τb.[cast_calculus.types.TRec τb/])>>). by apply back_closed.
+    eapply rewrite_typed.
+    eapply Fold_typed. eapply PI_Γ_typed. eapply rewrite_typed. apply IHtyped.
+    rewrite back_unfold_comm. auto. auto.
+  - eapply Unfold_typed_help. by rewrite back_unfold_comm.
+    eapply rewrite_typed. by apply IHtyped. by simpl.
+  - destruct (decide (cons_stand_open τi τf)); destruct (decide (cast_calculus.types.TClosed τi)); destruct (decide (cast_calculus.types.TClosed τf)); try by contradiction.
     eapply App_typed.
-    rewrite /𝓕c /env_subst. admit.
+    apply EClosed_typed. apply 𝓕c_closed; auto.
+    rewrite /𝓕c /env_subst. asimpl. eapply force_typed. apply 𝓕_typed. auto. auto.
     apply IHtyped.
-  - apply Ω_typed. admit.
-Admitted.
-
-From fae_gtlc_mu.embedding Require Export types.
-
-Lemma well_typedness_ctx_item Γ τ Γ' τ' C :
-  cast_calculus.contexts.typed_ctx_item C Γ τ Γ' τ' →
-  typed_ctx_item (backtranslate_ctx_item C) (map backtranslate_type Γ) (backtranslate_type τ) (map backtranslate_type Γ') (backtranslate_type τ').
-Proof.
-  induction 1; try (by constructor).
-  - apply TP_CTX_AppL. apply well_typedness_expr; done.
-  - apply TP_CTX_AppR.
-    assert (triv : backtranslate_type (types.TArrow τ τ') = TArrow <<τ>> <<τ'>>). by simpl. rewrite -triv. clear triv.
-    by apply well_typedness_expr.
-  - constructor. by apply well_typedness_expr.
-  - constructor. by apply well_typedness_expr.
-  - constructor.
-    assert (triv : backtranslate_type τ1 :: (map backtranslate_type Γ) = map backtranslate_type (τ1 :: Γ)). by simpl. rewrite triv. clear triv.
-      by apply well_typedness_expr.
-    assert (triv : backtranslate_type τ2 :: (map backtranslate_type Γ) = map backtranslate_type (τ2 :: Γ)). by simpl. rewrite triv. clear triv.
-      by apply well_typedness_expr.
-  - apply TP_CTX_CaseM with (τ2 := <<τ2>>).
-    assert (triv : backtranslate_type (types.TSum τ1 τ2) = TSum <<τ1>> <<τ2>>). by simpl. rewrite -triv. clear triv.
-      by apply well_typedness_expr.
-    assert (triv : backtranslate_type τ2 :: (map backtranslate_type Γ) = map backtranslate_type (τ2 :: Γ)). by simpl. rewrite triv. clear triv.
-      by apply well_typedness_expr.
-  - apply TP_CTX_CaseR with (τ1 := <<τ1>>).
-    assert (triv : backtranslate_type (types.TSum τ1 τ2) = TSum <<τ1>> <<τ2>>). by simpl. rewrite -triv. clear triv.
-      by apply well_typedness_expr.
-    assert (triv : backtranslate_type τ1 :: (map backtranslate_type Γ) = map backtranslate_type (τ1 :: Γ)). by simpl. rewrite triv. clear triv.
-      by apply well_typedness_expr.
-  - rewrite unfolding_backtranslation_commutes. apply TP_CTX_Fold.
-  - rewrite unfolding_backtranslation_commutes. apply TP_CTX_Unfold.
-  - simpl. destruct (cons_stand_dec τi τf); destruct (decide (TClosed τi)); destruct (decide (TClosed τf)); try by contradiction.
-    eapply TP_CTX_AppR. admit.
-Admitted.
-
-Lemma well_typedness_ctx Γ τ Γ' τ' C :
-  cast_calculus.contexts.typed_ctx C Γ τ Γ' τ' →
-  typed_ctx (backtranslate_ctx C) (map backtranslate_type Γ) (backtranslate_type τ) (map backtranslate_type Γ') (backtranslate_type τ').
-Proof.
-  induction 1.
-  - constructor.
-  - econstructor; simpl. by apply well_typedness_ctx_item.
-    auto.
+  - apply Ω_typed.
+  Unshelve.
+   try by apply back_closed.
+   try by apply back_closed.
+   try by apply back_closed.
+   cut (TClosed (<<(cast_calculus.types.TRec τb)>>)). by simpl.
+   by apply back_closed.
+   by rewrite back_unfold_comm in HC.
+   cut (TClosed (<<(cast_calculus.types.TRec τb)>>)). by simpl.
+   by apply back_closed.
+   cut (TClosed (<<(cast_calculus.types.TArrow τi τf)>>)). by simpl.
+   apply back_closed. by apply cast_calculus.types.TArrow_closed.
+   auto.
+   auto.
+   auto.
 Qed.
+
+(* From fae_gtlc_mu.embedding Require Export types. *)
+
+(* Lemma well_typedness_ctx_item Γ τ Γ' τ' C : *)
+(*   cast_calculus.contexts.typed_ctx_item C Γ τ Γ' τ' → *)
+(*   typed_ctx_item (backtranslate_ctx_item C) (map backtranslate_type Γ) (backtranslate_type τ) (map backtranslate_type Γ') (backtranslate_type τ'). *)
+(* Proof. *)
+(*   induction 1; try (by constructor). *)
+(*   - apply TP_CTX_AppL. apply well_typedness_expr; done. *)
+(*   - apply TP_CTX_AppR. *)
+(*     assert (triv : backtranslate_type (types.TArrow τ τ') = TArrow <<τ>> <<τ'>>). by simpl. rewrite -triv. clear triv. *)
+(*     by apply well_typedness_expr. *)
+(*   - constructor. by apply well_typedness_expr. *)
+(*   - constructor. by apply well_typedness_expr. *)
+(*   - constructor. *)
+(*     assert (triv : backtranslate_type τ1 :: (map backtranslate_type Γ) = map backtranslate_type (τ1 :: Γ)). by simpl. rewrite triv. clear triv. *)
+(*       by apply well_typedness_expr. *)
+(*     assert (triv : backtranslate_type τ2 :: (map backtranslate_type Γ) = map backtranslate_type (τ2 :: Γ)). by simpl. rewrite triv. clear triv. *)
+(*       by apply well_typedness_expr. *)
+(*   - apply TP_CTX_CaseM with (τ2 := <<τ2>>). *)
+(*     assert (triv : backtranslate_type (types.TSum τ1 τ2) = TSum <<τ1>> <<τ2>>). by simpl. rewrite -triv. clear triv. *)
+(*       by apply well_typedness_expr. *)
+(*     assert (triv : backtranslate_type τ2 :: (map backtranslate_type Γ) = map backtranslate_type (τ2 :: Γ)). by simpl. rewrite triv. clear triv. *)
+(*       by apply well_typedness_expr. *)
+(*   - apply TP_CTX_CaseR with (τ1 := <<τ1>>). *)
+(*     assert (triv : backtranslate_type (types.TSum τ1 τ2) = TSum <<τ1>> <<τ2>>). by simpl. rewrite -triv. clear triv. *)
+(*       by apply well_typedness_expr. *)
+(*     assert (triv : backtranslate_type τ1 :: (map backtranslate_type Γ) = map backtranslate_type (τ1 :: Γ)). by simpl. rewrite triv. clear triv. *)
+(*       by apply well_typedness_expr. *)
+(*   - rewrite back_unfold_comm. apply TP_CTX_Fold. *)
+(*   - rewrite back_unfold_comm. apply TP_CTX_Unfold. *)
+(*   - simpl. destruct (cons_stand_dec τi τf); destruct (decide (TClosed τi)); destruct (decide (TClosed τf)); try by contradiction. *)
+(*     eapply TP_CTX_AppR. admit. *)
+(* Admitted. *)
+
+(* Lemma well_typedness_ctx Γ τ Γ' τ' C : *)
+(*   cast_calculus.contexts.typed_ctx C Γ τ Γ' τ' → *)
+(*   typed_ctx (backtranslate_ctx C) (map backtranslate_type Γ) (backtranslate_type τ) (map backtranslate_type Γ') (backtranslate_type τ'). *)
+(* Proof. *)
+(*   induction 1. *)
+(*   - constructor. *)
+(*   - econstructor; simpl. by apply well_typedness_ctx_item. *)
+(*     auto. *)
+(* Qed. *)
