theories/refinements/static_gradual/compat_cast/all.v
@@ -1,4 +1,4 @@
-From fae_gtlc_mu.refinements.static_gradual Require Export tactics_left logical_relation resources_right compat_easy help_left compat_cast.defs.
+From fae_gtlc_mu.refinements.static_gradual Require Export logical_relation resources_right compat_easy help_left compat_cast.defs.
 From fae_gtlc_mu.cast_calculus Require Export types typing.
 From fae_gtlc_mu.stlc_mu Require Export lang.
 From fae_gtlc_mu.cast_calculus Require Export lang.
@@ -6,9 +6,10 @@ From iris.algebra Require Import list.
 From iris.proofmode Require Import tactics.
 From iris.program_logic Require Import lifting.
 From fae_gtlc_mu.cast_calculus Require Export types.
-From fae_gtlc_mu.cast_calculus Require Export consistency.structural.definition.
+From fae_gtlc_mu.cast_calculus Require Export consistency.structural.
 From fae_gtlc_mu.backtranslation Require Export cast_help.general cast_help.extract cast_help.embed.
-From fae_gtlc_mu.refinements.static_gradual.compat_cast Require Export between_rec star_ground ground_star tau_star star_tau prod_prod sum_sum arrow_arrow identity.
+From fae_gtlc_mu.refinements.static_gradual.compat_cast Require Export between_rec prod_prod sum_sum arrow_arrow identity tau_star ground_star tau_star star_tau.
+(*    star_ground *)
 
 Section compat_cast_all.
   Context `{!implG Σ,!specG Σ}.
@@ -27,44 +28,46 @@ Section compat_cast_all.
   Lemma back_cast_ar_all {A} {τi τf} (pC : cons_struct A τi τf) : back_cast_ar pC.
   Proof.
     induction pC.
-    - by apply back_cast_ar_star_ground.
+    (* - by apply back_cast_ar_star_ground. *)
+    - admit.
     - by apply back_cast_ar_ground_star.
-    - apply back_cast_ar_tau_star.
-    - apply back_cast_ar_star_tau.
-    - apply back_cast_ar_base_base.
-    - apply back_cast_ar_star_star.
+    - by apply back_cast_ar_tau_star.
+    - by apply back_cast_ar_star_tau.
+    - by apply back_cast_ar_base_base.
+    - by apply back_cast_ar_star_star.
     - by apply back_cast_ar_sum_sum.
     - by apply back_cast_ar_prod_prod.
     - by apply back_cast_ar_arrow_arrow.
     - by apply back_cast_ar_trec_trec_expose.
     - by apply back_cast_ar_trec_trec_use.
-  Qed.
+  Admitted.
+
 
   Notation "'` H" := (bin_log_related_alt H) (at level 8).
 
-  Lemma interp_closed Δ τ (pτc : TClosed τ) :
-    ⟦ τ ⟧ Δ
-    ≡ ⟦ τ ⟧ [].
-  Proof. Admitted.
+  (* Lemma interp_closed Δ τ (pτc : TClosed τ) : *)
+  (*   ⟦ τ ⟧ Δ *)
+  (*   ≡ ⟦ τ ⟧ []. *)
+  (* Proof. Admitted. *)
 
-  Lemma interp_closed' Δ τ vv' (pτc : TClosed τ) :
-    ⟦ τ ⟧ Δ vv'
-    ≡ ⟦ τ ⟧ [] vv'.
-  Proof. Admitted.
+  (* Lemma interp_closed' Δ τ vv' (pτc : TClosed τ) : *)
+  (*   ⟦ τ ⟧ Δ vv' *)
+  (*   ≡ ⟦ τ ⟧ [] vv'. *)
+  (* Proof. Admitted. *)
 
 
-  Lemma bin_log_related_back_cast Γ e e' τi τf (pC : cons_struct [] τi τf) (pτic : TClosed τi) (pτfc : TClosed τf)
+  Lemma bin_log_related_back_cast Γ e e' τi τf (pC : cons_struct [] τi τf)
       (IHHtyped : Γ ⊨ e ≤log≤ e' : τi) :
     Γ ⊨ 𝓕c pC [] e ≤log≤ Cast e' τi τf : τf.
   Proof.
-    iIntros (Δ vvs ei ?) "#[Hρ HΓ]"; iIntros (K) "Hj /=".
+    iIntros (vvs ei) "#[Hρ HΓ]"; iIntros (K) "Hj /=".
     rewrite 𝓕c_closed; try auto.
     rewrite 𝓕c_rewrite.
     iApply (wp_bind (fill [stlc_mu.lang.AppRCtx _])).
-    iApply (wp_wand with "[Hj]"). iApply ('`IHHtyped _ _ _ (CastCtx τi τf :: K)). iFrame. auto.
+    iApply (wp_wand with "[Hj]"). iApply ('`IHHtyped _ _ (CastCtx τi τf :: K)). iFrame. auto.
     iIntros (v). iDestruct 1 as (v') "[Hv' Hvv']". simpl.
     rewrite -𝓕c_rewrite.
-    rewrite (interp_closed' _ τi); auto.
+    (* rewrite (interp_closed' _ τi); auto. *)
     iApply (wp_wand with "[-]").
     iApply ((back_cast_ar_all pC) with "[-]").
     iSplitR. unfold rel_cast_functions. iSplit; auto.
@@ -73,16 +76,14 @@ Section compat_cast_all.
     iIntros (v). iDestruct 1 as (v') "[Hv' Hvv']".
     iExists v'.
     auto.
-    rewrite (interp_closed' Δ τf). auto. auto.
-  Admitted.
-
+    Unshelve. apply hack.
+  Qed.
 
   Lemma bin_log_related_omega Γ e' τ :
     Γ ⊨ Ω ≤log≤ e' : τ.
   Proof.
-    iIntros (Δ vvs ρ ?) "#[Hρ HΓ]"; iIntros (K) "Hj /=".
+    iIntros (vvs ρ) "#[Hρ HΓ]"; iIntros (K) "Hj /=".
     by iApply wp_Ω.
   Qed.
-
 
 End compat_cast_all.
