theories/refinements/static_gradual/compat_cast/between_rec.v
@@ -1,10 +1,10 @@
-From fae_gtlc_mu.refinements.static_gradual Require Export logical_relation resources_right compat_easy help_left compat_cast.defs tactics_left.
+From fae_gtlc_mu.refinements.static_gradual Require Export logical_relation resources_right compat_easy help_left compat_cast.defs.
 From fae_gtlc_mu.cast_calculus Require Export types typing.
 From fae_gtlc_mu.cast_calculus Require Export lang.
 From iris.algebra Require Import list.
 From iris.proofmode Require Import tactics.
 From iris.program_logic Require Import lifting.
-From fae_gtlc_mu.cast_calculus Require Export consistency.structural.definition.
+From fae_gtlc_mu.cast_calculus Require Export consistency.structural.
 From fae_gtlc_mu.backtranslation Require Export cast_help.general cast_help.extract cast_help.embed.
 From fae_gtlc_mu.cast_calculus Require Export lang types.
 (* From iris.program_logic Require Import language. *)
@@ -26,17 +26,17 @@ Section between_rec.
   (* Implicit Types a : (cast_calculus.types.type * cast_calculus.types.type). *)
   Local Hint Resolve to_of_val : core.
 
-  Lemma interp_subst Δ2 τ τ' v : ⟦ τ ⟧ (⟦ τ' ⟧ Δ2 :: Δ2) v ≡ ⟦ τ.[τ'/] ⟧ Δ2 v.
-  Proof. apply (interp_subst_up []). Qed.
+  (* Lemma interp_subst Δ2 τ τ' v : ⟦ τ ⟧ (⟦ τ' ⟧ Δ2 :: Δ2) v ≡ ⟦ τ.[τ'/] ⟧ Δ2 v. *)
+  (* Proof. apply (interp_subst_up []). Qed. *)
 
   (* Lemma compat_cast_between_TRec A τl τr (p : (TRec τl, TRec τr) ∉ A) (pC : cons_struct ((TRec τl, TRec τr) :: A) ). *)
 
   (** Proving it *)
 
-  Lemma refold_interp_unknown' vv' : fixpoint interp_unknown1' vv' ≡ interp TUnknown [] vv'.
-  Proof.
-    auto.
-  Qed.
+  (* Lemma refold_interp_unknown' vv' : fixpoint interp_unknown1' vv' ≡ interp TUnknown [] vv'. *)
+  (* Proof. *)
+  (*   auto. *)
+  (* Qed. *)
 
   Lemma back_cast_ar_trec_trec_use:
     ∀ (A : list (type * type)) (τl τr : {bind type}) (i : nat) (pμτlμtrinA : A !! i = Some (TRec τl, TRec τr)),
@@ -79,25 +79,26 @@ Section between_rec.
 
   Lemma back_cast_ar_trec_trec_expose:
     ∀ (A : list (type * type)) (τl τr : {bind type}) (pμτlμτrnotA : (TRec τl, TRec τr) ∉ A)
-      (pC : ((TRec τl, TRec τr) :: A) ⊢ τl.[TRec τl/] ~ τr.[TRec τr/]) (IHpC : back_cast_ar pC),
+      (pC : cons_struct ((TRec τl, TRec τr) :: A) τl.[TRec τl/] τr.[TRec τr/]) (IHpC : back_cast_ar pC),
       back_cast_ar (consTRecTRecExposeCall A τl τr pμτlμτrnotA pC).
   Proof.
     intros A τl τr pμτlμτrnotA pC IHpC.
     rewrite /𝓕c /𝓕 /back_cast_ar; iIntros (ei' K' v v' fs) "(#Hfs & #Hvv' & #Hei' & Hv')".
     (** setting up iLöb *)
     iLöb as "IHlob" forall (v v' ei' K') "Hvv' Hei'".
-    fold (𝓕c (consTRecTRecExposeCall A τl τr pμτlμτrnotA pC) fs).
+    (* fold (𝓕c (consTRecTRecExposeCall A τl τr pμτlμτrnotA pC) fs). *)
     (* iRevert (ei' K' v v') "Hvv' Hei' Hv'". *)
     rewrite {2}/𝓕c. rewrite /𝓕.
     fold (𝓕 pC).
     (** rewriting value relation for v and v' *)
-    rewrite fixpoint_interp_rec1_eq.
-    iDestruct "Hvv'" as ([w w']) "#[% Hww']".
+    (* rewrite fixpoint_interp_rec1_eq. *)
+    rewrite interp_rw_TRec.
+    iDestruct "Hvv'" as (w w') "#[% Hww']".
     inversion H; clear v v' H H1 H2.
     fold interp.
-    fold (interp_rec ⟦ τl ⟧ []).
-    assert (bydef : interp_rec ⟦ τl ⟧ [] = ⟦ TRec τl ⟧ []); auto; rewrite bydef. clear bydef.
-    rewrite (interp_subst [] τl (TRec τl) (w, w')).
+    (* fold (interp_rec ⟦ τl ⟧ []). *)
+    (* assert (bydef : interp_rec ⟦ τl ⟧ [] = ⟦ TRec τl ⟧ []); auto; rewrite bydef. clear bydef. *)
+    (* rewrite (interp_subst [] τl (TRec τl) (w, w')). *)
     (** evaluation steps in WP *)
     (* applying to value v *)
     iApply wp_pure_step_later; auto; iNext.
@@ -105,7 +106,7 @@ Section between_rec.
     rewrite rewrite_subs_app.
     do 2 rewrite Fix_subs_rewrite.
     assert (triv :
-              Fix (stlc_mu.lang.Lam (stlc_mu.lang.Lam (stlc_mu.lang.Fold (rename (+1) (𝓕 pC).[upn 1 (ren (+1))] (stlc_mu.lang.Unfold (stlc_mu.lang.Var 0)))))).[up (stlc_mu.typing.env_subst fs)].[stlc_mu.lang.of_val $ stlc_mu.lang.FoldV w/] (stlc_mu.lang.Var 0).[up (stlc_mu.typing.env_subst fs)].[stlc_mu.lang.of_val $ stlc_mu.lang.FoldV w/] = Fix (stlc_mu.lang.Lam (stlc_mu.lang.Lam (stlc_mu.lang.Fold ((𝓕 pC).[up (stlc_mu.typing.env_subst fs) >> ren (+1)] (stlc_mu.lang.Unfold (ids 0)))))) (stlc_mu.lang.Fold (w))). by asimpl. rewrite triv. clear triv.
+              Fix (stlc_mu.lang.Lam (stlc_mu.lang.Lam (stlc_mu.lang.Fold ((𝓕 pC).[upn 1 (ren (+1))].[ren (+1)] (stlc_mu.lang.Unfold (stlc_mu.lang.Var 0)))))).[up (stlc_mu.typing.env_subst fs)].[stlc_mu.lang.of_val $ stlc_mu.lang.FoldV w/] (stlc_mu.lang.Var 0).[up (stlc_mu.typing.env_subst fs)].[stlc_mu.lang.of_val $ stlc_mu.lang.FoldV w/] = Fix (stlc_mu.lang.Lam (stlc_mu.lang.Lam (stlc_mu.lang.Fold ((𝓕 pC).[up (stlc_mu.typing.env_subst fs) >> ren (+1)] (stlc_mu.lang.Unfold (ids 0)))))) (stlc_mu.lang.Fold (w))). by asimpl. rewrite triv. clear triv.
     (* evaluation step of the Fix itself *)
     iApply (wp_bind (stlc_mu.lang.fill_item $ stlc_mu.lang.AppLCtx _)).
     iApply wp_fix''.
@@ -191,14 +192,12 @@ Section between_rec.
     iApply wp_value.
     iExists (FoldV v').
     iFrame.
-    rewrite fixpoint_interp_rec1_eq.
+    rewrite interp_rw_TRec.
     simpl. iModIntro.
-    iExists (v , v').
-    iSplitR. done.
-    iNext.
-    by rewrite (interp_subst [] τr (TRec τr) (v, v')).
-    (* trival shells here *)
-  Admitted.
+    iExists v , v'.
+    iSplitR. done. auto.
+    Unshelve. all:apply hacki.
+  Qed.
 
 
 End between_rec.
