theories/refinements/static_gradual/compat_cast/defs.v
@@ -46,6 +46,8 @@ Section defs.
   (** The statement that the -- closed up -- back-translated casts behave appropriately.
       (We redefine it here to a new statement, making it a bit more amenable for proving.) *)
 
+  (* TODO!! 𝓕cV instead of 𝓕c *)
+
   Definition back_cast_ar {A} {τi τf} (pC : cons_struct A τi τf) :=
   ∀ ei' K' v v' fs, (rel_cast_functions A fs ∗ ⟦ τi ⟧ (v, v') ∗ initially_inv ei' ∗ currently_half (fill K' (Cast (cast_calculus.lang.of_val v') τi τf)))
                      ⊢ (WP (𝓕c pC fs (stlc_mu.lang.of_val v)) {{ w, ∃ w', currently_half (fill K' (cast_calculus.lang.of_val w')) ∗ ⟦ τf ⟧ (w, w') }})%I.
