theories/refinements/static_gradual/compat_cast/ground_star.v
@@ -21,68 +21,47 @@ Section ground_star.
   Local Hint Resolve to_of_val : core.
   Local Hint Resolve stlc_mu.lang.to_of_val : core.
 
-  (* Lemma refold_interp_unknown' vv' : fixpoint interp_unknown1' vv' ≡ interp TUnknown [] vv'. *)
-  (* Proof. *)
-  (*   auto. *)
-  (* Qed. *)
-
-
   Lemma back_cast_ar_ground_star:
     ∀ (A : list (type * type)) (τG : type) (G : Ground τG), back_cast_ar (consTGroundStar A τG G).
   Proof.
     intros A τG G.
     rewrite /back_cast_ar /𝓕c /𝓕. iIntros (ei' K' v v' fs) "(#Hfs & #Hvv' & #Hei' & Hv')". rewrite embed_no_subs.
     destruct G; rewrite /𝓕c /𝓕.
-      + rewrite interp_rw_TUnit. iDestruct "Hvv'" as "%". simpl in H. inversion H. rewrite H0 H1. clear v v' H H0 H1.
-        wp_head. asimpl. wp_value.
-        iExists (CastV UnitV _ _ (TGround_TUnknown_icp Ground_TUnit)). iSplitL. done.
-        rewrite interp_rw_TUnknown. iExists _, _. simpl. iModIntro.
-        iLeft. simpl. done. constructor.
-      + iDestruct "Hvv'" as ((v1 , v1') (v2 , v2')) "[% [H1 H2]]". simpl in H; inversion H; clear H H1 H2 v v'.
-        wp_head. asimpl. wp_value.
-        iExists (CastV (PairV v1' v2') _ _ (TGround_TUnknown_icp _ Ground_TProd)). iSplitL. done.
-        rewrite (unfold_fixpoint_interp_unknown1' [] (stlc_mu.lang.FoldV (stlc_mu.lang.InjLV (stlc_mu.lang.InjLV (stlc_mu.lang.InjRV (stlc_mu.lang.PairV v1 v2)))),
-    CastV (PairV v1' v2') (⋆ × ⋆) ⋆ (TGround_TUnknown_icp (⋆ × ⋆) Ground_TProd))).
-        iModIntro. iRight. iLeft.
-        iExists v1 , v1' , v2 , v2'. iSplit. done. iSplit; done.
       + wp_head. asimpl. wp_value.
-        iExists (CastV v' _ _ (TGround_TUnknown_icp _ Ground_TSum)).
-        iSplitL. done. rewrite unfold_fixpoint_interp_unknown1'.
+        iExists (CastV v' _ _ (TGround_TUnknown_icp Ground_TUnit)). iSplitL. done.
+        rewrite interp_rw_TUnknown. iExists _, _.
+        iLeft. iModIntro. iSplit; done.
+      + wp_head. asimpl. wp_value.
+        iExists (CastV v' _ _ (TGround_TUnknown_icp Ground_TProd)). iSplitL. done.
+        rewrite interp_rw_TUnknown.
+        iExists _  , _.
+        iModIntro. iRight. iLeft. iSplit; done.
+      + wp_head. asimpl. wp_value.
+        iExists (CastV v' _ _ (TGround_TUnknown_icp Ground_TSum)).
+        iSplitL. done.
+        (* rewrite unfold_fixpoint_interp_unknown1'. *)
+        rewrite interp_rw_TUnknown.
+        iExists v, v'.
         iModIntro. iRight. iRight. iLeft.
-        iDestruct "Hvv'" as "[H1 | H2]".
-        * iDestruct "H1" as ((v1 , v1')) "[% H1]".
-          simpl in H; inversion H; clear H H1 H2 v v'.
-          iLeft. iExists v1 , v1'. iSplit. done. auto.
-        * iDestruct "H2" as ((v2 , v2')) "[% H2]".
-          simpl in H; inversion H; clear H H1 H2 v v'.
-          iRight. iExists v2 , v2'. iSplit. done. auto.
-        * constructor.
-      + iDestruct "Hvv'" as "#Hvv'". wp_head. asimpl. wp_value.
-        iExists (CastV v' _ _ (TGround_TUnknown_icp _ Ground_TArrow)). iSplitL. done.
-        rewrite unfold_fixpoint_interp_unknown1'.
-        iModIntro. iRight. iRight. iRight. iLeft.
-        iExists v , v'. iSplit. done. iModIntro. iModIntro.
-        iIntros (a a').
-        fold (interp_unknown_pre').
-        fold (interp_unknown' [] (a , a')).
-        fold (interp ⋆).
-        iIntros "#Haa'".
-        clear K'. iIntros (K') "Hv'a'".
-        iApply ("Hvv'" $! (a , a') with "Haa' Hv'a'"). constructor.
+        iSplit; auto.
+      + wp_head. asimpl. wp_value.
+        iExists (CastV v' _ _ (TGround_TUnknown_icp Ground_TArrow)). iSplitL. done.
+        rewrite interp_rw_TUnknown.
+        iExists _ , _.
+        iModIntro. iRight. iRight. iRight. iLeft. iSplitL; done.
       + wp_head. asimpl.
         (** rewriting value relation for v and v' *)
-        rewrite fixpoint_interp_rec1_eq.
-        iDestruct "Hvv'" as ([u u']) "#[% Huu']". inversion H. clear v v' H H1 H2.
-        (** boring steps *)
+        rewrite interp_rw_TRec.
+        iDestruct "Hvv'" as (u u') "#[% Huu']". inversion H. clear v v' H H1 H2.
         iApply (wp_bind (fill $ [stlc_mu.lang.InjRCtx ; stlc_mu.lang.FoldCtx])).
         wp_head. wp_value. simpl. wp_value.
-        iExists (CastV (FoldV u') _ _ (TGround_TUnknown_icp _ Ground_TRec)).
+        iExists (CastV (FoldV u') _ _ (TGround_TUnknown_icp Ground_TRec)).
         iSplitL. done.
-        rewrite (unfold_fixpoint_interp_unknown1' [] (stlc_mu.lang.FoldV (stlc_mu.lang.InjRV u), CastV (FoldV u') (TRec ⋆) ⋆ (TGround_TUnknown_icp (TRec ⋆) Ground_TRec))).
-        iModIntro. iRight. iRight. iRight. iRight.
-        iExists u , u'. iSplit; done.
-        (* Unshelve. apply (@ectx_lang_ctx stlc_mu.lang.ectx_lang _). *)
-  Admitted.
+        rewrite (interp_rw_TUnknown (stlc_mu.lang.FoldV _ , _)).
+        iExists _ , _.
+        iModIntro. iRight. iRight. iRight. iRight. iSplit; done.
+        Unshelve. apply hack.
+  Qed.
 
 
 End ground_star.
