theories/refinements/static_gradual/compat_cast/tau_star.v
@@ -1,13 +1,13 @@
-From fae_gtlc_mu.refinements.static_gradual Require Export tactics_left logical_relation resources_right compat_easy help_left compat_cast.defs.
+From fae_gtlc_mu.refinements.static_gradual Require Export logical_relation resources_right compat_easy help_left compat_cast.defs.
 From fae_gtlc_mu.cast_calculus Require Export types typing.
 From fae_gtlc_mu.stlc_mu Require Export lang.
 From fae_gtlc_mu.cast_calculus Require Export lang.
 From iris.algebra Require Import list.
 From iris.proofmode Require Import tactics.
 From iris.program_logic Require Import lifting.
-From fae_gtlc_mu.cast_calculus Require Export consistency.structural.definition.
+From fae_gtlc_mu.cast_calculus Require Export consistency.structural.
 From fae_gtlc_mu.backtranslation Require Export cast_help.general cast_help.extract cast_help.embed.
-From fae_gtlc_mu.cast_calculus Require Export types.
+From fae_gtlc_mu.cast_calculus Require Export lang types.
 
 Section compat_cast_tau_star.
   Context `{!implG Σ,!specG Σ}.
@@ -24,18 +24,28 @@ Section compat_cast_tau_star.
   (** Proving it *)
 
   Lemma back_cast_ar_tau_star:
-    ∀ (A : list (type * type)) (τ τG : type) (pτnG : Ground τ → False) (pτnStar : τ ≠ ⋆) 
-      (pτSτG : get_shape τ = Some τG) (pC : A ⊢ τ ~ τG), back_cast_ar (consTauStar A τ τG pτnG pτnStar pτSτG pC).
+    ∀ (A : list (type * type)) (τ τG : type) (pτnG : Ground τ → False) (pτnStar : τ ≠ ⋆) (pτSτG : get_shape τ = Some τG) (pC1 : cons_struct A τ τG) (pC2 : cons_struct A τG ⋆),
+      back_cast_ar pC1 → back_cast_ar pC2 → back_cast_ar (consTauStar A τ τG pτnG pτnStar pτSτG pC1 pC2).
   Proof.
-    intros A τ τG pτnG pτnStar pτSτG pC.
-    rewrite /back_cast_ar /𝓕c /𝓕. iIntros (ei' K' v v' fs) "(#Hfs & #Hvv' & #Hei' & Hv')".
-    fold (𝓕 pC).
-    wp_head. asimpl. rewrite embed_no_subs.
-    (** IH *)
-    (* embed is a value.. *)
-    admit.
-    (* iApply (wp_bind (fill $ [stlc_mu.lang.AppRCtx _])). *)
-    (** embedding stuff *)
-  Admitted.
+    intros A τ τG pτnG pτnStar pτSτG pC1 pC2 IHpC1 IHpC2.
+    rewrite /back_cast_ar /𝓕c /𝓕. fold (𝓕 pC1). fold (𝓕 pC2).
+    iIntros (ei' K' v v' fs) "(#Hfs & #Hvv' & #Hei' & Hv')".
+    iDestruct "Hfs" as "[% Hfs']"; iAssert (rel_cast_functions A fs) with "[Hfs']" as "Hfs". iSplit; done. iClear "Hfs'".
+    wp_head. asimpl.
+    fold (𝓕c pC1 fs). fold (𝓕c pC2 fs). do 2 rewrite 𝓕c_rewrite.
+    iApply (wp_bind (fill $ [stlc_mu.lang.AppRCtx _])).
+    iApply (wp_wand with "[-]").
+    iMod (step_pure _ ei' K'
+                    (Cast (# v') τ ⋆)
+                    (Cast (Cast (# v') τ τG) τG ⋆) with "[Hv']") as "Hv'"; auto.
+    { eapply UpFactorization; auto. by eapply get_shape_is_ground. }
+    rewrite -𝓕c_rewrite.
+    iApply (IHpC1 ei' (CastCtx τG ⋆ :: K') with "[Hv']"); auto.
+    iIntros (w) "blaa".  iDestruct "blaa" as (w') "[Hw' #Hww']".
+    simpl.
+    rewrite -𝓕c_rewrite.
+    iApply (IHpC2 ei' K' with "[Hw']"); auto.
+    Unshelve. apply hack.
+  Qed.
 
 End compat_cast_tau_star.
